dev2020/dsubsup_cc/cc2cc.v
@@ -1,0 +1,302 @@
+Require Import List PeanoNat.
+Import Notations.
+
+Axiom proof_irrelevance: forall {P: Prop} (p1 p2: P), p1 = p2.
+
+(* Variables and Contexts *)
+Definition fVar : Set := nat.
+
+Definition bVar : Set := nat.
+
+Inductive var : Set :=
+  | varB : bVar -> var
+  | varF : fVar -> var.
+
+Notation "# i" := (varB i) (at level 0) : var_scope.
+Notation "` x" := (varF x) (at level 0) : var_scope.
+Notation "g ~ T" := (cons T g) (at level 50) : var_scope.
+Notation "g +~ g'" := (g' ++ g) (at level 60) : var_scope.
+
+Bind Scope var_scope with var.
+Open Scope var_scope.
+
+(* Lookup -- de Bruijn levels *)
+Inductive lookup {ty} : list ty -> fVar -> ty -> Prop :=
+  | last : forall g T, lookup (g ~ T) (length g) T
+  | prev : forall g T U x, lookup g x T -> lookup (g ~ U) x T.
+
+
+Inductive sort: Set := prop | type.
+
+Inductive expr : Set :=
+  | TSort : sort -> expr
+  | tVar : var -> expr
+  | TAll : expr -> expr -> expr
+  | tLam : expr -> expr
+  | tApp : expr -> expr -> expr
+  | TSig : expr -> expr -> expr
+  | tPair : expr -> expr -> expr
+  | tFst : expr -> expr
+  | tSnd : expr -> expr.
+
+Definition cx := list expr.
+
+Coercion TSort: sort >-> expr.
+Coercion tVar: var >-> expr.
+
+(* Opening *)
+Reserved Notation "e{ i :-> x }" (at level 50).
+Fixpoint open (i : bVar) (e' e : expr) : expr :=
+  match e with
+  | tVar #j => if i =? j then e' else #j
+  | TSort _ | tVar `_ => e
+  | TAll T U => TAll (e{i :-> e'} T) (e{S i :-> e'} U)
+  | tLam t => tLam (e{S i :-> e'} t)
+  | tApp t u => tApp (e{i :-> e'} t) (e{i :-> e'} u)
+  | TSig T U => TSig (e{i :-> e'} T) (e{S i :-> e'} U)
+  | tPair t u => tPair (e{i :-> e'} t) (e{i :-> e'} u)
+  | tFst t => tFst (e{i :-> e'} t)
+  | tSnd t => tSnd (e{i :-> e'} t)
+  end
+  where "e{ i :-> e' }" := (open i e').
+
+Notation "e *^ u" := (open 0 u e) (at level 50).
+
+Reserved Notation "e ~~> u" (no associativity, at level 90).
+
+Compute (e{0 :-> tVar (varF 1)} (tLam (varB 2))).
+
+(* Closed expressions *)
+Inductive closed (b f : nat) : expr -> Prop :=
+  | cl_sort : forall s : sort, closed b f s
+  | cl_varF : forall x, x < f -> closed b f `x
+  | cl_varB : forall i, i < b -> closed b f #i
+  | cl_all : forall T U, 
+      closed b f T -> closed (S b) f U -> closed b f (TAll T U)
+  | cl_lam : forall e, closed (S b) f e -> closed b f (tLam e)
+  | cl_app : forall t u,
+      closed b f t -> closed b f u -> closed b f (tApp t u)
+  | cl_sig : forall T U,
+      closed b f T -> closed (S b) f U -> closed b f (TSig T U)
+  | cl_pair : forall t u,
+      closed b f t -> closed b f u -> closed b f (tPair t u)
+  | cl_fst : forall t, closed b f t -> closed b f (tFst t)
+  | cl_snd : forall t, closed b f t -> closed b f (tSnd t).
+
+Reserved Notation "e ~~> u" (no associativity, at level 90).
+Inductive reduce : expr -> expr -> Prop :=
+  | r_beta : forall e u, tApp (tLam e) u ~~> e *^ u
+  | r_eta : forall e, (tLam (tApp e #0)) ~~> e
+  | r_pi1 : forall e u, tFst (tPair e u) ~~> e
+  | r_pi2 : forall e u, tSnd (tPair e u) ~~> u
+  | r_all1 : forall T U T', T ~~> T' -> TAll T U ~~> TAll T' U
+  | r_all2 : forall T U U', U ~~> U' -> TAll T U ~~> TAll T U'
+  | r_lam : forall e e', e ~~> e' -> tLam e ~~> tLam e'
+  | r_app1 : forall e u e', e ~~> e' -> tApp e u ~~> tApp e' u
+  | r_app2 : forall e u u', u ~~> u' -> tApp e u ~~> tApp e u'
+  | r_sig1 : forall T U T', T ~~> T' -> TSig T U ~~> TSig T' U
+  | r_sig2 : forall T U U', U ~~> U' -> TSig T U ~~> TSig T U'
+  (* The lecture notes linked above don't mention adding these 
+     substructural rules for pairs, but I think they're required, else
+     we can't reduce inside tuples. *)
+  | r_pair1 : forall t u t', t ~~> t' -> tPair t u ~~> tPair t' u
+  | r_pair2 : forall t u u', u ~~> u' -> tPair t u ~~> tPair t u'
+  | r_fst : forall t t', t ~~> t' -> tFst t ~~> tFst t'
+  | r_snd : forall t t', t ~~> t' -> tSnd t ~~> tSnd t'
+   where "e ~~> u" := (reduce e u).
+
+Reserved Notation "e == u" (at level 90, no associativity).
+Inductive equals: expr -> expr -> Prop :=
+  | e_red: forall {e u}, e ~~> u -> e == u
+  | e_refl: forall {e}, e == e
+  | e_sym: forall {e u}, e == u -> u == e
+  | e_trans: forall {e u t}, e == u -> u == t -> e == t
+  where "e == u" := (equals e u).
+
+Inductive hasType: cx -> expr -> expr -> Prop :=
+  | t_ax: forall {g}, wfCx g -> hasType g prop type
+
+  | t_var: 
+      forall {g}, wfCx g ->
+      forall {x T}, lookup g x T ->
+      hasType g `x T
+
+  | t_all:
+      forall {g T sT}, hasType g T (TSort sT) ->
+      forall {U sU}, hasType (g ~ T) (U *^ varF (length g)) (TSort sU) ->
+      closed 1 (length g) U ->
+      hasType g (TAll T U) sU
+
+  | t_lam: 
+      forall {g T s}, hasType g T (TSort s) ->
+      forall {e U}, hasType (g ~ T) (e *^ ` (length g)) (U *^ ` (length g)) ->
+      closed 0 (length g) (TAll T U) ->
+      closed 1 (length g) e ->
+      hasType g (tLam e) (TAll T U)
+
+  | t_app:
+      forall {g e T U}, hasType g e (TAll T U) ->
+      forall {u}, hasType g u T ->
+      hasType g (tApp e u) (U *^ u)
+
+  | t_sig:
+      forall {g T sT}, hasType g T (TSort sT) ->
+      forall {U sU}, hasType (g ~ T) (U *^ varF (length g)) (TSort sU) ->
+      closed 1 (length g) U ->
+      hasType g (TSig T U) sU
+
+  | t_pair:
+      forall {g T U s}, hasType g (TSig T U) (TSort s) ->
+      forall {t}, hasType g t T ->
+      forall {u}, hasType g u (U *^ t) ->
+      hasType g (tPair t u) (TSig T U)
+
+  | t_fst: 
+      forall {g e T U}, hasType g e (TSig T U) -> 
+      hasType g (tFst e) T
+
+  | t_snd:
+      forall {g e T U}, hasType g e (TSig T U) ->
+      hasType g (tSnd e) (U *^ tFst e)
+
+  | t_conv:
+      forall {g e T}, hasType g e T ->
+      forall {U}, T == U ->
+      forall {s}, hasType g U (TSort s) ->
+      hasType g e U
+
+  with wfCx: cx -> Prop :=
+  | wf_nil: wfCx nil
+  | wf_snoc: 
+      forall {g T s}, hasType g T (TSort s) -> 
+      wfCx (g ~ T).
+
+Theorem hasType_closed: 
+  forall {g: cx} {e T}, hasType g e T ->
+  closed 0 (length g) e /\ closed 0 (length g) T.
+Admitted.
+
+Theorem hasType_wfCx:
+  forall {g e T}, hasType g e T -> wfCx g.
+Admitted.
+
+Inductive Cx: forall {g}, wfCx g -> cx -> Prop :=
+  | tr_nil: Cx wf_nil nil
+
+  | tr_cons: 
+      forall {g T s} {wfT: hasType g T (TSort s)}
+      {g' T' s'}, Expr wfT g' T' (TSort s') ->
+      Cx (wf_snoc wfT) (g' ~ T')
+
+  with Expr: forall {g e T}, hasType g e T -> cx -> expr -> expr -> Prop :=
+  | tr_ax: 
+      forall {g} {G: wfCx g} {g'}, Cx G g' ->
+      Expr (t_ax G) g' prop type
+
+  | tr_var:
+      forall {g T s} {wfT: hasType g T (TSort s)} 
+      {g' T' s'}, Expr wfT g' T' (TSort s') ->
+      forall {x} (lx: lookup g x T), 
+      Expr (t_var (hasType_wfCx wfT) lx) g' `x T'
+
+  | tr_all:
+      forall {g T sT} {wfT: hasType g T (TSort sT)} {g' T' sT'}, 
+      Expr wfT g' T' (TSort sT') ->
+      forall {U sU} {wfU: hasType (g ~ T) (U *^ ` (length g)) (TSort sU)}
+      {U' sU'}, Expr wfU (g' ~ T') (U' *^ ` (length g')) (TSort sU') ->
+      forall (cl: closed 1 (length g) U),
+      Expr (t_all wfT wfU cl) g' (TAll T' U') sU'
+
+  | tr_lam:
+      forall {g T sT} {wfT: hasType g T (TSort sT)} {g' T' sT'}, 
+      Expr wfT g' T' (TSort sT') ->
+      forall {U sU} {wfU: hasType (g ~ T) (U *^ ` (length g)) (TSort sU)}
+      {U' sU'}, Expr wfU (g' ~ T') (U' *^ ` (length g')) (TSort sU') ->
+      forall {e} {eT: hasType (g ~ T) (e *^ ` (length g)) (U *^ ` (length g))},
+      forall {e'}, Expr eT (g' ~ T') (e' *^ ` (length g)) (U' *^ ` (length g)) ->
+      forall {cl1: closed 0 (length g) (TAll T U)} {cl2: closed 1 (length g) e},
+      Expr (@t_lam _ _ _ wfT e U eT cl1 cl2) g' (tLam e') (TAll T' U')
+
+  | tr_app:
+      forall {g T sT} {wfT: hasType g T (TSort sT)} {g' T' sT'}, 
+      Expr wfT g' T' (TSort sT') ->
+      forall {U sU} {wfU: hasType g U (TSort sU)} {U' sU'}, 
+      Expr wfU g' U' (TSort sU') ->
+      forall {e} {eTU: hasType g e (TAll T U)} {e'},
+      Expr eTU g' e' (TAll T' U') ->
+      forall {u} {uT: hasType g u T} {u'},
+      Expr uT g' u' T' ->
+      Expr (t_app eTU uT) g' (tApp e' u') U'
+
+  | tr_sig:
+      forall {g T sT} {wfT: hasType g T (TSort sT)} {g' T' sT'}, 
+      Expr wfT g' T' (TSort sT') ->
+      forall {U sU} {wfU: hasType (g ~ T) (U *^ ` (length g)) (TSort sU)}
+      {U' sU'}, Expr wfU (g' ~ T') (U' *^ ` (length g')) (TSort sU') ->
+      forall (cl: closed 1 (length g) U),
+      Expr (t_all wfT wfU cl) g' (TSig T' U') sU'
+
+  | tr_pair:
+      forall {g T U s} {wfp: hasType g (TSig T U) (TSort s)} {g' T' U' s'},
+      Expr wfp g' (TSig T' U') (TSort s') ->
+      forall {t} {tT: hasType g t T} {t'},
+      Expr tT g' t' T' ->
+      forall {u} {uU: hasType g u (U *^ t)} {u'},
+      Expr uU g' u' (U' *^ t') ->
+      Expr (t_pair wfp tT uU) g' (tPair t' u') (TSig T' U')
+
+  | tr_fst:
+      forall {g e T U} {eT: hasType g e (TSig T U)} {g' e' T' U'},
+      Expr eT g' e' (TSig T' U') ->
+      Expr (t_fst eT) g' (tFst e') T'
+  
+  | tr_snd:
+      forall {g e T U} {eT: hasType g e (TSig T U)} {g' e' T' U'},
+      Expr eT g' e' (TSig T' U') ->
+      Expr (t_snd eT) g' (tSnd e') (U' *^ tFst e').
+
+Theorem Expr_Cx: 
+  forall {g e T} {eT: hasType g e T} {g' e' T'}, Expr eT g' e' T' ->
+  Cx (hasType_wfCx eT) g'.
+Proof.
+  induction 1. 
+  - assert (hasType_wfCx (t_ax G) = G). apply proof_irrelevance.
+    rewrite H0. assumption.
+  - assert (hasType_wfCx (t_var (hasType_wfCx wfT)))
+
+Theorem tr_cx_length: 
+  forall {g} {G: wfCx g} {g'}, Cx G g' -> length g = length g'.
+Proof.
+  induction 1; auto. simpl. 
+
+Fixpoint tr_expr
+  {g e T} {eT: hasType g e T}
+  {g' e' T'} (etr: Expr eT g' e' T')
+  : hasType g' e' T'
+
+  with tr_cx
+  {g} {G: wfCx g} {g'} (cxtr: Cx G g')
+  : wfCx g'
+Proof.
+  * destruct etr.
+    - constructor. eapply tr_cx; eassumption.
+    - constructor. eapply hasType_wfCx. eapply tr_expr; eassumption.
+      admit (* lookup *).
+    - econstructor. eapply tr_expr. eassumption. eapply tr_expr. eassumption.
+      admit (* closed *).
+    - econstructor. eapply tr_expr. eassumption. eapply tr_expr. 
+      assert (length g = length g') by admit. rewrite <- H. eassumption.
+      admit. admit.
+    - assert (U' = U' *^ u') by admit. rewrite H. econstructor.
+      eapply tr_expr. eassumption. eapply tr_expr. eassumption.
+    - econstructor. eapply tr_expr. eassumption. eapply tr_expr. eassumption.
+      admit (* closed *).
+    - econstructor. eapply tr_expr. eassumption. eapply tr_expr. eassumption.
+      eapply tr_expr. eassumption.
+    - econstructor. eapply tr_expr. eassumption.
+    - econstructor. eapply tr_expr. eassumption.
+
+  * destruct G.
+    - inversion ctr. constructor.
+    - eapply tr_cx. eassumption.
+Admitted.
