dev2020/dsubsup_cc/d2cc4.v
@@ -1,0 +1,43 @@
+Require Import List.
+
+Definition fVar : Set := nat.
+
+Definition bVar : Set := nat.
+
+Inductive var : Set :=
+  | varB : bVar -> var
+  | varF : fVar -> var.
+
+Notation "# i" := (varB i) (at level 0).
+Notation "` x" := (varF x) (at level 0).
+Notation "G ~ T" := (cons T G) (at level 50).
+Notation "G +~ G'" := (G' ++ G) (at level 60).
+
+Bind Scope var_scope with var.
+Open Scope var_scope.
+
+Module CC.
+
+  (* Presyntax *)
+  Inductive sort : Set := prop | type.
+
+  Inductive expr : Set :=
+    | TSort : sort -> expr
+    | tVar : var -> expr
+    | TAll : expr -> expr -> expr
+    | tLam : expr -> expr
+    | tApp : expr -> expr -> expr
+    | TSig : expr -> expr -> expr
+    | tPair : expr -> expr -> expr
+    | tFst : expr -> expr
+    | tSnd : expr -> expr.
+
+  Definition cx := list expr.
+  Definition env := list expr.
+
+  Notation "t $" := (tApp t) (at level 4).
+  Notation "t & u" := (tPair t u) (at level 4).
+  Coercion TSort : sort >-> expr.
+  Coercion tVar : var >-> expr.
+
+  
